+++
title = "Extended Euclidian Algorithm Explained"
date = "2025-10-12T00:00:00+00:00"
tags = ["math", "algorithm", "python"]
description = "Explanation and implementation of the extended euclidian algorithm in python"
math = true
+++

In this blog post, I explain the Euclidian Algorithm (+extended) and how to implement them in python.

## Prerequisite: Modulus Operator

First, we need to understand the modulus operator.

The modulus operator, often represented by the percent character (`%`) in many programming languages, returns the rest of the division between 2 operands.

For example, let's say we have 2 integers `a=5` and `b=2`. Then `a mod b` will be equal to `1`

```bash
~ â¯ python3
Python 3.13.7 (main, Aug 14 2025, 00:00:00) [GCC 14.3.1 20250523 (Red Hat 14.3.1-1)] on linux
Type "help", "copyright", "credits" or "license" for more information.
>>> a=5
>>> b=2
>>> a%b
1
```

We can also think of it as:

> How much would remain if we put the maximum possible number of `b`s inside `a` ?

In our example, `q=2` is the maximum number of times we can fit `b` into `a` without going over. And the remainder (to reach the value of a) is `r=1`. This can be seen in the below figure:

{{<figure src="/img/general/ext_euclid_alg/modulus_explain_1.png" position=center caption="Visual Representation">}}

This gives the following relation: \[ a = bq + r \]

## Euclidian Algorithm
  
The Euclidian algorithm is used to get the **Greatest Common Divisor** `d` of 2 integers `a` and `b` (ie. the biggest number that divides both `a` and `b`).

\[ d = gcd(a,b) \]

In order to find the gcd, the algorithm relies on the following claim:

> if `a` and `b` are both divisible by `d`, then `r = a mod b` is also divisible by `d`

but how can we prove it ?

**Approach 1: math**

What we know: both `a` and `b` are divisible by `d`.

What we are trying to prove: `r = a mod b` is also divisible by `d`.


> **Info** \
> An integer `x` being divisible by another integer `y` means that `x` can be written: $$ x = ny $$ where `n` is also an integer.

Knowing this, `a` and `b` could be written:

$$
a = nd \\
b = md
$$

Using this and the earlier formula (`a=bq+r`) we get:

$$
r = a - bq \\
r = (nd) - (md)q \\
r = (n - mq) * d
$$

`r` can be written as an integer (`n-mq`) times `d`, therefore `r` is divisible by `d`.

**Approach 2: visual intuition**

In this approach, we need to think of `x` being divisible by `y` as `x` being made of `n` blocks of size `y` (x, y, n integers).

{{<figure src="/img/general/ext_euclid_alg/blocks_illustration.png" position=center caption="Blocks illustration">}}

In the above figure, we see that `a` is made of `n` blocks of size `d` and `b` is made of `m` blocks of size `d`. This is the same as `a=n*d` and `b=m*d`

In this illustration, we can see that the remainder `r` will always be made up of a **whole** number of blocks of size `d`, thus will always be divisible by `d`. This is because `r` is what remains when you substract `b` "`q` times" from `a` (ie. `r = a - bq`) and since `a` and `b` are made of the same unit blocks, naturally the remainder will also be the same.

Now coming back to the Euclidian Algorithm.

We have shown that if `a` and `b` are divisible by `d`, then `r = a mod b` is also divisible by `d`.

And we know that `a` and `b` are both divisible by `gcd(a,b)`, which means that `r = a mod b` is also divisible by `gcd(a,b)`.

So `r`, being smaller than `a` and `b`, will naturally have the same gcd as them.

We can therefore write:

$$
gcd(a,b) = gcd(a,r) = gcd(b,r)
$$

This helps a lot in reducing the possibilities, since finding the gcd for smaller numbers is easier that larger ones.

### Implementation

The algorithm will first compute `r = a % b`.

If `r` is equal to 0, it will return `min(a,b)`

Else it will return `gcd(min(a,b), r)`

```python
def gcd(a, b):
    r = a % b

    if r == 0:
        return min(a, b)

    return gcd(min(a, b), r)

print(gcd(12,44))
```


## Extended Euclidian Algorithm

The extended euclidan algorithm is a way to find 2 integers `x` and `y` such that:

$$
x * a+y * b=gcd(a,b)
$$

To start, let's look at the simplest case first: when `r=0`.

If we are given 2 integers `a` and `b` (`a` > `b`) and `r = a % b = 0`, then `b` (the smallest) is the gcd.

In this case, `x` would be `0` and `y` would be `1`:

$$
0*a+1*b=gcd(a,b)=b
$$

This will be the base case of the recursion.

Now let's try to understand the different steps involved.

{{<figure src="/img/general/ext_euclid_alg/recursion_steps.png" position=center caption="Recursion Steps">}}

At the start, we are given 2 integers `A0` and `B0` (`A0` > `B0`) and we are trying to find:
- `d = gcd(A0, B0)`
- `x` and `y` such that $$x*A0+y*B0=d$$

At step 0, we compute `r0 = A0 % B0`, if it's not `0` we move to step 1 with `A1 = B0` and `B1 = r0`.

At step 1, we repeat the same until we reach step n.

At step n, we compute `rn = An % Bn` and find that it is equal to `0`. We have reached the base case, so we return `d=Bn, x=0, y=1`:

$$
d = B_n = 0*An + 1*Bn
$$

Then, we go back to step n-1. Here we need to recalculate x and y for `An-1` and `Bn-1`, because the previous values we had were for `An` and `Bn`. For each step we need to have right values of `x` and `y`, until we ultimately get back to step 0 where we'll have the final values.

We can generalize this problem in the following manner:

> Knowing the values `x` and `y` for step k, what are the values for step k-1 ?

From the arrows in the illustration, we can see:
- `Ak = Bk-1`
- `Bk = rk-1 = Ak-1 - Bk-1 * qk-1`

Knowing this, we can find the new values of `x` and `y`:

$$
d = xA_k + yB_k \\
d = xB_{k-1} + y r_{k-1} \\
d = xB_{k-1} + y(A_{k-1} - B_{k-1}q_{k-1}) \\
d = xB_{k-1} + yA_{k-1} - yB_{k-1}q_{k-1} \\
d = yA_{k-1} + (x - yq_{k-1})B_{k-1}
$$

In the end we have:

$$
x_{k-1} = y_{k} \\
y_{k-1} = x - yq_{k-1}
$$

### Implementation

We now have everything we need to implement the algorithm.

```python
def f(a, b):
    # Calculating the remainder
    r = a % b

    # Base case
    if r == 0:
        arr = [b, 0, 1]
        return arr

    else:
        arr = f(b, r)

        # Calculating the new values of x and y
        new_x = arr[2]
        new_y = arr[1] - arr[2] * (a//b)

        arr = [arr[0], new_x, new_y]
        return arr


a = 12
b = 44
res = f(a, b)
print(f"{res[0]} = {res[1]} * {a} + {res[2]} * {b}")
```
